Add object type check in normal form

src/NRGTNF.v
@@ -15,38 +15,42 @@ Require Import SchemaWellFormedness.
 Require Import Schema.
 Require Import SchemaAux.
 
+Require Import QueryConformance.
+
 Require Import CpdtTactics.
 
 Section NRGTNF.
 
   Variables Name Vals : ordType.
-  
+
+  Implicit Type schema : @wfSchema Name Vals.
   Implicit Type queries : seq (@Query Name Vals).
   Implicit Type query : @Query Name Vals.
   Definition is_field := @is_field Name Vals.
   Definition is_inline_fragment := @is_inline_fragment Name Vals.
 
 
-  Equations is_in_normal_form (query : @Query Name Vals) : bool :=
+  Equations is_in_normal_form schema (query : @Query Name Vals) : bool :=
     {
-      is_in_normal_form (NestedField _ _ ϕ) := (all is_field ϕ || all is_inline_fragment ϕ) && all is_in_normal_form ϕ;
-      is_in_normal_form (NestedLabeledField _ _ _ ϕ) := (all is_field ϕ || all is_inline_fragment ϕ) && all is_in_normal_form ϕ;
-      is_in_normal_form (InlineFragment _ ϕ) := (all is_field ϕ) && all is_in_normal_form ϕ;
-      is_in_normal_form _ := true
+      is_in_normal_form schema (NestedField _ _ ϕ) := (all is_field ϕ || all is_inline_fragment ϕ) && all (is_in_normal_form schema) ϕ;
+      is_in_normal_form schema (NestedLabeledField _ _ _ ϕ) := (all is_field ϕ || all is_inline_fragment ϕ) && all (is_in_normal_form schema) ϕ;
+      is_in_normal_form schema (InlineFragment t ϕ) := [&& (is_object_type schema t), (all is_field ϕ) & all (is_in_normal_form schema) ϕ];
+      is_in_normal_form _ _ := true
     }.
   
-  Definition are_in_normal_form (queries : seq (@Query Name Vals)) : bool :=
-    (all is_field queries || all is_inline_fragment queries) && all is_in_normal_form queries.
+  Definition are_in_normal_form schema (queries : seq (@Query Name Vals)) : bool :=
+    (all is_field queries || all is_inline_fragment queries) && all (is_in_normal_form schema) queries.
 
 
-  Lemma are_in_normal_form_E queries :
-    are_in_normal_form queries ->
-    (all is_field queries \/ all is_inline_fragment queries) /\ all is_in_normal_form queries.
+  Lemma are_in_normal_form_E schema queries :
+    are_in_normal_form schema queries ->
+    (all is_field queries \/ all is_inline_fragment queries) /\ all (is_in_normal_form schema) queries.
   Proof.
     rewrite /are_in_normal_form.
     by move/andP=> [/orP H H'].
   Qed.
-  
+
+ 
   Fixpoint no_repeated_query (queries : list (@Query Name Vals)) : bool :=
      match queries with
         | [::] => true
@@ -68,6 +72,11 @@ Section NRGTNF.
   Definition are_non_redundant (queries : seq (@Query Name Vals)) : bool :=
     no_repeated_query queries && all is_non_redundant queries.
 
+  Lemma are_non_redundantE (queries : seq (@Query Name Vals)) :
+    are_non_redundant queries ->
+    no_repeated_query queries /\ all is_non_redundant queries.
+  Proof. by rewrite /are_non_redundant; move/andP. Qed.
+  
   Lemma is_are_non_redundant_nf n α ϕ :
     is_non_redundant (NestedField n α ϕ) = are_non_redundant ϕ.
   Proof. done. Qed.
@@ -79,6 +88,39 @@ Section NRGTNF.
   Lemma is_are_non_redundant_if t ϕ :
     is_non_redundant (InlineFragment t ϕ) = are_non_redundant ϕ.
   Proof. done. Qed.
-      
 
+  Lemma non_redundant_inv (queries : seq (@Query Name Vals)) :
+    no_repeated_query queries ->
+    all is_non_redundant queries ->
+    are_non_redundant queries.
+  Proof.
+      by move=> Hnrep Hnr; rewrite /are_non_redundant; apply/andP.
+  Qed.
+
+  Lemma adf schema ty ϕ :
+    is_object_type schema ty ->
+    all (query_conforms schema ty) ϕ ->
+    all is_inline_fragment ϕ ->
+    are_non_redundant ϕ ->
+    exists ϕ', ϕ = [:: InlineFragment ty ϕ'].
+  Proof.
+    funelim (is_object_type schema ty) => // _.
+  Admitted.
+
+  Lemma sub_nf schema ty ϕ ϕ' :
+    ϕ = [:: InlineFragment ty ϕ'] ->
+    are_in_normal_form schema ϕ ->
+    all is_field ϕ' /\ all (is_in_normal_form schema) ϕ'.
+  Proof.
+    move=> -> H.
+    move: (are_in_normal_form_E H) => [_ Hnf].
+    move: Hnf; rewrite {1}/all is_in_normal_form_equation_5.
+      by move/andP=> [/and3P [Hobj Hfld H'] _].
+  Qed.
+
+  Lemma sub_nr schema ty ϕ ϕ' :
+    ϕ = [:: InlineFragment ty ϕ'] ->
+    are_non_redundant schema ϕ ->
+    all (are_non_redundant schema) ϕ'.
+  
 End NRGTNF.
